progs64/verif_incr_atomic.v
@@ -52,10 +52,10 @@ Definition thread_func_spec :=
   WITH y : val, x : namespace * share * share * lock_handle * lock_handle * gname * gname * gname * globals
   PRE [ tptr tvoid ]
          let '(i, sh1, sh, l, ht, g, g1, g2, gv) := x in
-         PROP  (readable_share sh1; ptr_of ht = y)
+         PROP  (readable_share sh1; ptr_of ht = y; i ## name_of l)
          PARAMS (y) GLOBALS (gv)
          SEP   (inv i (cptr_inv g g1 g2); lock_inv sh l (ctr_inv gv g); field_at sh1 t_counter [StructField _lock] (ptr_of l) (gv _c);
-                ghost_var gsh2 O g1; lock_inv sh ht (thread_lock_inv sh1 sh gv l g g1 ht))
+                ghost_var gsh2 O g1; lock_inv sh ht (thread_lock_inv sh1 sh gv l g g1 (ghost_of ht)))
   POST [ tint ]
          PROP ()
          RETURN (Vint Int.zero)
@@ -89,15 +89,6 @@ Proof.
 Qed.
 #[local] Hint Resolve thread_inv_exclusive : core.
 
-(* up *)
-Lemma ghost_var_update' : forall {A} g (v1 v2 v : A), ghost_var gsh1 v1 g * ghost_var gsh2 v2 g |--
-  |==> !!(v1 = v2) && (ghost_var gsh1 v g * ghost_var gsh2 v g).
-Proof.
-  intros; erewrite ghost_var_share_join' by eauto.
-  Intros; subst; erewrite ghost_var_share_join by eauto.
-  rewrite -> prop_true_andp by auto; apply ghost_var_update.
-Qed.
-
 Lemma body_incr: semax_body Vprog Gprog f_incr incr_spec.
 Proof.
   start_function.
@@ -125,8 +116,8 @@ Proof.
     iExists tt; iDestruct "ctr_state" as "[g' $]".
     rewrite add_repr.
     iMod (ghost_var_update' with "[$g' $g]") as "(-> & g1 & g2)".
-    unfold ctr_inv at 1; iSplitL "ctr g2"; [iExists (n + 1)%nat; iFrame|].
-    { rewrite Nat2Z.inj_add; auto. }
+    iSplitL "ctr g2".
+    { iExists (n + 1)%nat; rewrite Nat2Z.inj_add; iFrame; auto. }
     iModIntro; iSplit.
     { (* tactic? *)
       iIntros "[inv l]". unfold ctr_inv at 1.
@@ -191,19 +182,18 @@ Qed.
    but this wouldn't allow us to deallocate the lock at the end. *)
 
 (* prove a lemma about our specific use pattern of incr *)
-Lemma incr_inv_shift : forall i gv sh g l g1 g2 gvar, (gvar = g1 \/ gvar = g2) ->
+Lemma incr_inv_shift : forall i gv sh g l g1 g2 gvar, (gvar = g1 \/ gvar = g2) -> i ## name_of l ->
   lock_inv sh l (ctr_inv gv g) * inv i (cptr_inv g g1 g2) * ghost_var gsh2 0%nat gvar |--
-  atomic_shift (λ n : nat, ctr_state gv (ptr_of l) g n) ⊤ ∅
+  atomic_shift (λ n : nat, ctr_state gv (ptr_of l) g n) (⊤ ∖ ∅) ∅
       (λ (n : nat) (_ : ()), fold_right_sepcon [ctr_state gv (ptr_of l) g (n + 1)%nat]) (λ _ : (), lock_inv sh l (ctr_inv gv g) * ghost_var gsh2 1%nat gvar).
 Proof.
   intros.
-  unfold lock_inv; simpl; unfold atomic_lock_inv.
-  destruct l as ((v, i0), g0); Intros.
+  unfold_lock_inv; Intros.
   rewrite -> prop_true_andp by auto.
   iIntros "[[[#inv0 sh] #inv] g]".
   iAuIntro; rewrite /atomic_acc /=.
   iMod (into_acc_cinv with "inv0 sh") as (_) "[[>i sh] Hclose0]". done.
-  iInv "inv" as (x y) ">[[g1 g2] c]" "Hclose"; auto. admit. (* need to know the namespaces are distinct *)
+  iInv "inv" as (x y) ">[[g1 g2] c]" "Hclose"; auto.
   unfold ctr_state at 1.
   iExists (x + y)%nat; iFrame "c i sh inv0".
   iApply fupd_mask_intro; first by set_solver. iIntros "mask"; iSplit.
@@ -223,20 +213,18 @@ Proof.
       { iExists x, 1%nat; iFrame; auto.
         rewrite Nat.add_0_r; auto. }
       iApply "Hclose0"; auto.
-Admitted.
+Qed.
 
 Lemma body_thread_func : semax_body Vprog Gprog f_thread_func thread_func_spec.
 Proof.
   start_function.
   sep_apply lock_inv_isptr; Intros.
   forward_call (sh1, ptr_of l, g, gv, lock_inv sh l (ctr_inv gv g) * ghost_var gsh2 1%nat g1).
-  { sep_apply incr_inv_shift; auto.
-    replace (⊤ ∖ ∅) with (⊤ : coPset) by set_solver; cancel. }
+  { sep_apply incr_inv_shift; auto; cancel. }
   forward_call release_self (sh, ht, thread_lock_R sh1 sh gv l g g1).
-  { unfold thread_lock_inv, thread_lock_R, selflock; cancel. }
-  { (* type error? *) admit. }
+  { unfold thread_lock_inv, thread_lock_R; cancel. }
   forward.
-Admitted.
+Qed.
 
 Lemma body_main:  semax_body Vprog Gprog f_main main_spec.
 Proof.
@@ -260,27 +248,27 @@ Proof.
   unfold_data_at (data_at _ _ _ (gv _c)).
   rewrite <- 3(ghost_var_share_join gsh1 gsh2 Tsh) by auto with share; Intros.
   gather_SEP (atomic_int_at _ _ lockp) (field_at _ _ [StructField _ctr] _ _) (ghost_var gsh2 _ g);
-    viewshift_SEP 0 (EX h, !!(ptr_of h = lockp) && lock_inv Tsh h (ctr_inv gv g)).
+    viewshift_SEP 0 (EX lockg, lock_inv Tsh (lockp, nroot .@ "ctr", lockg) (ctr_inv gv g)).
   { go_lower; eapply derives_trans, make_lock_inv_0.
     unfold ctr_inv; Exists O; cancel. }
-  Intros lock; subst.
+  Intros lockg; set (lock := (lockp, nroot .@ "ctr", lockg)).
   (* need to split off shares for the locks here *)
   destruct split_Ews as (sh1 & sh2 & ? & ? & Hsh).
-  forward_call makelock_inv (gv, fun lockt => thread_lock_inv sh2 gsh2 gv lock g g1 lockt).
+  forward_call makelock_inv (gv, nroot .@ "tlock", fun lockt => thread_lock_inv sh2 gsh2 gv lock g g1 lockt).
   Intros lockt.
   match goal with |-context[|={⊤}=> ?P] => viewshift_SEP 1 P by entailer! end.
-  Intros ht; subst.
+  Intros gt; set (ht := (lockt, nroot .@ "tlock", gt)).
   sep_apply lock_inv_isptr; Intros.
   gather_SEP (ghost_var gsh1 _ g) (ghost_var gsh1 _ g1) (ghost_var gsh1 _ g2).
-  viewshift_SEP 0 (EX i : _, inv i (cptr_inv g g1 g2)).
+  viewshift_SEP 0 (inv (nroot .@ "ctr_inv") (cptr_inv g g1 g2)).
   { go_lower.
     eapply derives_trans, inv_alloc.
     eapply derives_trans, now_later.
     unfold cptr_inv.
     Exists O O; simpl; cancel. }
-  Intros i.
   rewrite invariant_dup; Intros.
-  forward_spawn _thread_func (ptr_of ht) (i, sh2, gsh2, lock, ht, g, g1, g2, gv).
+  assert (nroot.@"ctr_inv" ## nroot.@"ctr") by solve_ndisj.
+  forward_spawn _thread_func (ptr_of ht) (nroot .@ "ctr_inv", sh2, gsh2, lock, ht, g, g1, g2, gv).
   { entailer!.
     erewrite <- lock_inv_share_join; try apply gsh1_gsh2_join; auto.
     erewrite <- (lock_inv_share_join _ _ Tsh); try apply gsh1_gsh2_join; auto.
@@ -289,18 +277,16 @@ Proof.
   { simpl; auto. }
   rewrite invariant_dup; Intros.
   forward_call (sh1, ptr_of lock, g, gv, lock_inv gsh1 lock (ctr_inv gv g) * ghost_var gsh2 1%nat g2).
-  { sep_apply incr_inv_shift; auto.
-    replace (⊤ ∖ ∅) with (⊤ : coPset) by set_solver; cancel. }
-  forward_call acquire_inv_simple (gsh1, ht, thread_lock_inv sh2 gsh2 gv lock g g1 ht).
-  unfold thread_lock_inv at 2; unfold selflock, thread_lock_R; rewrite !later_sepcon; Intros.
+  { sep_apply incr_inv_shift; auto; cancel. }
+  forward_call acquire_inv_simple (gsh1, ht, thread_lock_inv sh2 gsh2 gv lock g g1 gt).
+  unfold thread_lock_inv at 2; unfold thread_lock_R; rewrite -> 3later_sepcon; Intros.
   forward_call (sh1, ptr_of lock, g, gv, fun n => !!(n = 2)%nat && lock_inv gsh1 lock (ctr_inv gv g) * ghost_var gsh2 1%nat g1).
-  { rewrite !sepcon_assoc; iIntros "(? & ? & ? & ? & g1 & lock & g2 & inv & ? & ? & ?)"; iSplitL "g1 g2 inv lock"; [|iVST; cancel_frame].
-    unfold lock_inv; simpl. unfold atomic_lock_inv. (* tactic *)
-    destruct lock as ((v, i0), g0). iDestruct "lock" as "[[[% %] #inv0] sh]".
+  { iIntros "(((((((? & g1) & lock) & g2) & inv) & ?) & ?) & ?)"; iSplitL "g1 g2 inv lock"; [|iVST; cancel_frame].
+    iDestruct "lock" as "[[[% %] #inv0] sh]".
     iDestruct "inv" as "#inv".
     iAuIntro; rewrite /atomic_acc /=.
     iMod (into_acc_cinv with "inv0 sh") as (_) "[[>i sh] Hclose0]". done.
-    iInv "inv" as (x y) ">[gs c]" "Hclose"; auto. admit. (* need to know the namespaces are distinct *)
+    iInv "inv" as (x y) ">[gs c]" "Hclose"; auto.
     iExists (x + y)%nat; iFrame "c i".
     iApply fupd_mask_intro; first set_solver.
     iFrame "sh".
@@ -332,14 +318,14 @@ Proof.
   forward_call acquire_inv_simple (gsh1, lock, ctr_inv gv g).
   forward_call freelock_self (gsh1, gsh2, ht, thread_lock_R sh2 gsh2 gv lock g g1).
   { lock_props.
-    unfold thread_lock_inv, thread_lock_R, selflock; cancel. }
+    unfold thread_lock_inv, thread_lock_R; subst ht; simpl; cancel. }
   unfold thread_lock_R; Intros.
   forward.
   forward_call freelock_simple (lock, ctr_inv gv g).
   { lock_props.
     erewrite <- (lock_inv_share_join gsh1 gsh2 Tsh); auto; cancel. }
   forward.
-Admitted.
+Qed.
 
 Definition extlink := ext_link_prog prog.
 
@@ -352,8 +338,10 @@ Proof.
 prove_semax_prog.
 repeat (apply semax_func_cons_ext_vacuous; [reflexivity | reflexivity | ]).
 semax_func_cons_ext.
-semax_func_cons_ext.
-semax_func_cons_ext.
+{ simpl; Intros p; unfold PROPx, LOCALx, SEPx, local; simpl; unfold liftx, lift1, lift; simpl; Intros; subst.
+  sep_apply atomic_int_isptr; Intros.
+  destruct ret; try contradiction.
+  unfold eval_id in *; simpl in *; apply prop_right; auto. }
 semax_func_cons_ext.
 semax_func_cons_ext.
 semax_func_cons_ext.
